dataplane/Examples/Collatz.thy
@@ -101,7 +101,7 @@ abbreviation "g4 inps \<equiv>
    comp_op_map (comp_op [Inr (nid4, p0) \<mapsto> Inr (nid0, p0)] (\<lambda> _. []) (inp_op nid4 inps) g3)"
 
 abbreviation "inps0 \<equiv> (\<lambda> p. llist_of []) :: 'a \<Rightarrow> (nat, nat \<times> nat) event llist"
-abbreviation "inps1 \<equiv> \<lambda> p. llist_of [Data (0 :: nat) (4 :: nat, 4 :: nat), Data 0 (2, 2)]"
+abbreviation "inps1 \<equiv> \<lambda> p. llist_of [Data (0 :: nat) (12 :: nat, 12 :: nat), Data 0 (2, 2)]"
 
 abbreviation "op \<equiv> g4 inps1"
 
@@ -130,7 +130,7 @@ definition "my_summ = (\<lambda> l1 l2.
 abbreviation \<open>sg \<equiv> init_subgraph my_summ (map (\<lambda> (nid, p). (Loc nid (Src p), bot, 1)) (List.product Enum.enum Enum.enum))\<close>
 abbreviation "dt \<equiv> dataflow_op sg op"
 
-definition "r = (trace_exec dt :: (unit, _ \<times> _, (nat \<times> nat) \<times> nat) VIO llist)"
+definition "r = (trace_exec dt :: (_, _ \<times> _, (nat \<times> nat) \<times> nat) VIO llist)"
 
 term DEBUG
 
